src/gopt/GSimulation.v
@@ -21,26 +21,25 @@ Set Implicit Arguments.
 Section Simulation.
   Definition SIM := forall (c1_src c1_tgt: Configuration.t), Prop.
 
-  Inductive _sim (sim: SIM) (c1_src c1_tgt:Configuration.t): Prop :=
-  | _sim_intro
-      (TERMINAL:
-         forall (TERMINAL_TGT: Threads.is_terminal c1_tgt.(Configuration.threads)),
-           <<TERMINAL_SRC: Threads.is_terminal c1_src.(Configuration.threads)>>)
-      (STEP:
-         forall e tid c3_tgt
-           (STEP_TGT: Configuration.step e tid c1_tgt c3_tgt),
-           <<ABORT: Configuration.steps_abort c1_src>> \/
-         exists c2_src c3_src,
-           <<STEPS_SRC: rtc Configuration.tau_step c1_src c2_src>> /\
-           <<STEP_SRC: Configuration.opt_step e tid c2_src c3_src>> /\
-           <<SIM: sim c3_src c3_tgt>>)
+  Definition _sim (sim: SIM) (c1_src c1_tgt:Configuration.t): Prop :=
+    forall (WF_SRC: Configuration.wf c1_src)
+      (WF_TGT: Configuration.wf c1_tgt),
+      <<TERMINAL:
+        forall (TERMINAL_TGT: Threads.is_terminal c1_tgt.(Configuration.threads)),
+          <<TERMINAL_SRC: Threads.is_terminal c1_src.(Configuration.threads)>>>> /\
+      <<STEP:
+        forall e tid c2_tgt
+          (STEP_TGT: Configuration.step e tid c1_tgt c2_tgt),
+        exists c2_src,
+          <<STEP_SRC: Configuration.opt_step e tid c1_src c2_src>> /\
+          <<SIM: sim c2_src c2_tgt>>>>
   .
 
   Lemma _sim_mon: monotone2 _sim.
   Proof.
-    ii. inv IN. econs; eauto. i.
-    exploit STEP; eauto. i. des; eauto.
-    right. esplits; eauto.
+    ii. exploit IN; eauto. i. des.
+    econs; eauto. ii.
+    exploit STEP; eauto. i. des. eauto.
   Qed.
   Hint Resolve _sim_mon: paco.
 
@@ -51,32 +50,32 @@ Hint Resolve _sim_mon: paco.
 
 Lemma sim_adequacy
       c_src c_tgt
+      (WF_SRC: Configuration.wf c_src)
+      (WF_TGT: Configuration.wf c_tgt)
       (SIM: sim c_src c_tgt):
   behaviors Configuration.step c_tgt <1= behaviors Configuration.step c_src.
 Proof.
-  i. revert c_src SIM.
+  i. revert c_src WF_SRC WF_TGT SIM.
   induction PR; i.
-  - punfold SIM0. inv SIM0. hexploit TERMINAL0; eauto. i. des.
+  - punfold SIM0. exploit SIM0; eauto. i. des.
+    hexploit TERMINAL0; eauto. i. des.
     econs 1. eauto.
-  - punfold SIM0. inv SIM0. exploit STEP0; eauto. i. des.
-    + inv ABORT. des.
-      eapply rtc_tau_step_behavior; eauto.
-      econs 3; eauto.
-    + inv SIM0; ss.
-      eapply rtc_tau_step_behavior; eauto.
-      inv STEP_SRC. econs 2; eauto.
-  - punfold SIM0. inv SIM0. exploit STEP0; eauto. i. des.
-    + inv ABORT. des.
-      eapply rtc_tau_step_behavior; eauto.
-      econs 3; eauto.
-    + inv SIM0; ss.
-      eapply rtc_tau_step_behavior; eauto.
-      inv STEP_SRC; eauto. econs 3; eauto.
-  - punfold SIM0. inv SIM0. exploit STEP0; eauto. i. des.
-    + inv ABORT. des.
-      eapply rtc_tau_step_behavior; eauto.
-      econs 3; eauto.
-    + inv SIM0; ss.
-      eapply rtc_tau_step_behavior; eauto.
-      inv STEP_SRC; eauto. econs 4; eauto.
+  - punfold SIM0. exploit SIM0; eauto. i. des.
+    exploit STEP0; eauto. i. des.
+    exploit Configuration.step_future; try exact STEP; eauto. i. des.
+    exploit Configuration.opt_step_future; try exact STEP_SRC; eauto. i. des.
+    inv SIM1; ss. inv STEP_SRC.
+    econs 2; eauto.
+  - punfold SIM0. exploit SIM0; eauto. i. des.
+    exploit STEP0; eauto. i. des.
+    exploit Configuration.step_future; try exact STEP; eauto. i. des.
+    exploit Configuration.opt_step_future; try exact STEP_SRC; eauto. i. des.
+    inv SIM1; ss. inv STEP_SRC.
+    econs 3; eauto.
+  - punfold SIM0. exploit SIM0; eauto. i. des.
+    exploit STEP0; eauto. i. des.
+    exploit Configuration.step_future; try exact STEP; eauto. i. des.
+    exploit Configuration.opt_step_future; try exact STEP_SRC; eauto. i. des.
+    inv SIM1; ss. inv STEP_SRC; eauto.
+    econs 4; eauto.
 Qed.
